LogicalRefinement/Typed/Wk.lean
@@ -83,6 +83,12 @@ theorem HasType.wk {Δ a A} (HΔ: Δ ⊢ a: A):
       apply HasVar.wk
       repeat assumption
 
+    case let_pair_iota => sorry
+
+    case let_set_iota => sorry
+
+    case let_repr_iota => sorry
+
     all_goals (
       intro ρ Γ R;
       rename_i' I5 I4 I3 I2 I1 I0;
